@prefix : <http://www.semanticweb.org/javi/ontologies/2025/3/tir#> .
@prefix owl: <http://www.w3.org/2002/07/owl#> .
@prefix rdf: <http://www.w3.org/1999/02/22-rdf-syntax-ns#> .
@prefix xml: <http://www.w3.org/XML/1998/namespace> .
@prefix xsd: <http://www.w3.org/2001/XMLSchema#> .
@prefix rdfs: <http://www.w3.org/2000/01/rdf-schema#> .
@base <http://www.semanticweb.org/javi/ontologies/2025/3/tir#> .

<http://www.semanticweb.org/javi/ontologies/2025/3/tir> rdf:type owl:Ontology ;
                                                         rdfs:comment "Ontology on smart tourism and recommendations"@en ;
                                                         rdfs:label "Tir" .

#################################################################
#    Annotation properties
#################################################################

###  http://swrl.stanford.edu/ontologies/3.3/swrla.owl#isRuleEnabled
<http://swrl.stanford.edu/ontologies/3.3/swrla.owl#isRuleEnabled> rdf:type owl:AnnotationProperty .


###  http://www.w3.org/2002/07/owl#sameAs
owl:sameAs rdf:type owl:AnnotationProperty .


#################################################################
#    Object Properties
#################################################################

###  http://www.semanticweb.org/javi/ontologies/2025/3/tir#eventLocatedIn
:eventLocatedIn rdf:type owl:ObjectProperty ;
                rdfs:domain :Event ;
                rdfs:range :City ;
                rdfs:comment "in which city is it located" ;
                rdfs:label "eventLocatedIn" .


###  http://www.semanticweb.org/javi/ontologies/2025/3/tir#hasGeoCoordinates
:hasGeoCoordinates rdf:type owl:ObjectProperty ;
                   owl:inverseOf :isGeoCoordinatesOf ;
                   rdfs:domain :City ;
                   rdfs:range :GeoCoordinates ;
                   rdfs:comment "has geographic coordinates" ;
                   rdfs:label "hasGeoCoordinates" .


###  http://www.semanticweb.org/javi/ontologies/2025/3/tir#hotelLocatedIn
:hotelLocatedIn rdf:type owl:ObjectProperty ;
                rdfs:domain :Hotel ;
                rdfs:range :City ;
                rdfs:comment "in which city is it located" ;
                rdfs:label "hotelLocatedIn" .


###  http://www.semanticweb.org/javi/ontologies/2025/3/tir#isGeoCoordinatesOf
:isGeoCoordinatesOf rdf:type owl:ObjectProperty ;
                    rdfs:domain :GeoCoordinates ;
                    rdfs:range :City ;
                    rdfs:comment "are geographic coordinates of" ;
                    rdfs:label "isGeoCoordinatesOf" .


###  http://www.semanticweb.org/javi/ontologies/2025/3/tir#restLocatedIn
:restLocatedIn rdf:type owl:ObjectProperty ;
               rdfs:domain :Restaurant ;
               rdfs:range :City ;
               rdfs:comment "in which city is it located" ;
               rdfs:label "restLocatedIn" .


###  http://www.semanticweb.org/javi/ontologies/2025/3/tir#tourLocatedIn
:tourLocatedIn rdf:type owl:ObjectProperty ;
               rdfs:domain :TouristAttraction ;
               rdfs:range :City ;
               rdfs:comment "in which city is it located" ;
               rdfs:label "tourLocatedIn" .


###  http://www.semanticweb.org/javi/ontologies/2025/3/tir#transLocatedIn
:transLocatedIn rdf:type owl:ObjectProperty ;
                rdfs:domain :PublicTransport ;
                rdfs:range :City ;
                rdfs:comment "in which city is it located" ;
                rdfs:label "transLocatedIn" .


#################################################################
#    Data properties
#################################################################

###  http://www.semanticweb.org/javi/ontologies/2025/3/tir#cityIdentifier
:cityIdentifier rdf:type owl:DatatypeProperty ;
                rdfs:domain :City ;
                rdfs:range xsd:int ;
                rdfs:comment "Unique city identifier" ;
                rdfs:label "cityIdentifier" .


###  http://www.semanticweb.org/javi/ontologies/2025/3/tir#cityName
:cityName rdf:type owl:DatatypeProperty ;
          rdfs:domain :City ;
          rdfs:range xsd:string ;
          rdfs:comment "name of each city" ;
          rdfs:label "cityName" .


###  http://www.semanticweb.org/javi/ontologies/2025/3/tir#eventIdentifier
:eventIdentifier rdf:type owl:DatatypeProperty ;
                 rdfs:domain :Event ;
                 rdfs:range xsd:int ;
                 rdfs:comment "Unique identifier of each event" ;
                 rdfs:label "eventIdentifier" .


###  http://www.semanticweb.org/javi/ontologies/2025/3/tir#eventName
:eventName rdf:type owl:DatatypeProperty ;
           rdfs:domain :Event ;
           rdfs:range xsd:string ;
           rdfs:comment "Name of each of the events" ;
           rdfs:label "eventName" .


###  http://www.semanticweb.org/javi/ontologies/2025/3/tir#hotelIdentifier
:hotelIdentifier rdf:type owl:DatatypeProperty ;
                 rdfs:domain :Hotel ;
                 rdfs:range xsd:int ;
                 rdfs:comment "Unique identifier of the hotels" ;
                 rdfs:label "hotelIdentifier" .


###  http://www.semanticweb.org/javi/ontologies/2025/3/tir#hotelName
:hotelName rdf:type owl:DatatypeProperty ;
           rdfs:domain :Hotel ;
           rdfs:range xsd:string ;
           rdfs:comment "Name of the hotels" ;
           rdfs:label "hotelName" .


###  http://www.semanticweb.org/javi/ontologies/2025/3/tir#hotelRatingValue
:hotelRatingValue rdf:type owl:DatatypeProperty ;
                  rdfs:domain :Hotel ;
                  rdfs:range xsd:decimal ;
                  rdfs:comment "Average rating of each hotel" ;
                  rdfs:label "hotelRatingValue" .


###  http://www.semanticweb.org/javi/ontologies/2025/3/tir#latitude
:latitude rdf:type owl:DatatypeProperty ;
          rdfs:domain :GeoCoordinates ;
          rdfs:range xsd:float ;
          rdfs:comment "latitude of the location" ;
          rdfs:label "latitude" .


###  http://www.semanticweb.org/javi/ontologies/2025/3/tir#legalName
:legalName rdf:type owl:DatatypeProperty ;
           rdfs:domain :PublicTransport ;
           rdfs:range xsd:string ;
           rdfs:comment "Legal name" ;
           rdfs:label "legalName" .


###  http://www.semanticweb.org/javi/ontologies/2025/3/tir#longitude
:longitude rdf:type owl:DatatypeProperty ;
           rdfs:domain :GeoCoordinates ;
           rdfs:range xsd:float ;
           rdfs:comment "longitude of the location" ;
           rdfs:label "longitude" .


###  http://www.semanticweb.org/javi/ontologies/2025/3/tir#pricePerNight
:pricePerNight rdf:type owl:DatatypeProperty ;
               rdfs:domain :Hotel ;
               rdfs:range xsd:decimal ;
               rdfs:comment "Hotel price per night" ;
               rdfs:label "pricePerNight" .


###  http://www.semanticweb.org/javi/ontologies/2025/3/tir#restAveragePrice
:restAveragePrice rdf:type owl:DatatypeProperty ;
                  rdfs:domain :Restaurant ;
                  rdfs:range xsd:decimal ;
                  rdfs:comment "Average restaurant bill price" ;
                  rdfs:label "restAveragePrice" .


###  http://www.semanticweb.org/javi/ontologies/2025/3/tir#restIdentifier
:restIdentifier rdf:type owl:DatatypeProperty ;
                rdfs:domain :Restaurant ;
                rdfs:range xsd:int ;
                rdfs:comment "Unique restaurant identifier" ;
                rdfs:label "restIdentifier" .


###  http://www.semanticweb.org/javi/ontologies/2025/3/tir#restName
:restName rdf:type owl:DatatypeProperty ;
          rdfs:domain :Restaurant ;
          rdfs:range xsd:string ;
          rdfs:comment "Name of the restaurants" ;
          rdfs:label "restName" .


###  http://www.semanticweb.org/javi/ontologies/2025/3/tir#restRatingValue
:restRatingValue rdf:type owl:DatatypeProperty ;
                 rdfs:domain :Restaurant ;
                 rdfs:range xsd:decimal ;
                 rdfs:comment "Average rating of each restaurant" ;
                 rdfs:label "restRatingValue" .


###  http://www.semanticweb.org/javi/ontologies/2025/3/tir#starRating
:starRating rdf:type owl:DatatypeProperty ;
            rdfs:domain :Hotel ;
            rdfs:range xsd:int ;
            rdfs:comment "star rating of each hotel" ;
            rdfs:label "starRating" .


###  http://www.semanticweb.org/javi/ontologies/2025/3/tir#startDate
:startDate rdf:type owl:DatatypeProperty ;
           rdfs:domain :Event ;
           rdfs:range xsd:dateTime ;
           rdfs:comment "evaluation of events" ;
           rdfs:label "starDate" .


###  http://www.semanticweb.org/javi/ontologies/2025/3/tir#tourIdentifier
:tourIdentifier rdf:type owl:DatatypeProperty ;
                rdfs:domain :TouristAttraction ;
                rdfs:range xsd:int ;
                rdfs:comment "Unique identifier for each of the city's tours" ;
                rdfs:label "tourIdentifier" .


###  http://www.semanticweb.org/javi/ontologies/2025/3/tir#tourName
:tourName rdf:type owl:DatatypeProperty ;
          rdfs:domain :TouristAttraction ;
          rdfs:range xsd:string ;
          rdfs:comment "Name of each of the tours" ;
          rdfs:label "tourName" .


###  http://www.semanticweb.org/javi/ontologies/2025/3/tir#tourRatingValue
:tourRatingValue rdf:type owl:DatatypeProperty ;
                 rdfs:domain :TouristAttraction ;
                 rdfs:range xsd:decimal ;
                 rdfs:comment "Average rating of each tour in the city" ;
                 rdfs:label "tourRatingValue" .


###  http://www.semanticweb.org/javi/ontologies/2025/3/tir#transAveragePrice
:transAveragePrice rdf:type owl:DatatypeProperty ;
                   rdfs:domain :PublicTransport ;
                   rdfs:range xsd:decimal ;
                   rdfs:comment "Average price of public transport in the city" ;
                   rdfs:label "transAveragePrice" .


###  http://www.semanticweb.org/javi/ontologies/2025/3/tir#transIdentifier
:transIdentifier rdf:type owl:DatatypeProperty ;
                 rdfs:domain :PublicTransport ;
                 rdfs:range xsd:int ;
                 rdfs:comment "Unique identifier of public transport in each city" ;
                 rdfs:label "transIdentifier" .


###  http://www.semanticweb.org/javi/ontologies/2025/3/tir#transName
:transName rdf:type owl:DatatypeProperty ;
           rdfs:domain :PublicTransport ;
           rdfs:range xsd:string ;
           rdfs:comment "Name of each public transport in the city" ;
           rdfs:label "transName" .


#################################################################
#    Classes
#################################################################

###  http://www.semanticweb.org/javi/ontologies/2025/3/tir#AndalusianRestaurant
:AndalusianRestaurant rdf:type owl:Class ;
                      rdfs:subClassOf :Restaurant ;
                      rdfs:comment "A public establishment where food and drinks, typically traditional Andalusian cuisine, are served on-site, with the aim of offering a culinary experience based on hospitality and the flavors of the region."@en ;
                      rdfs:label "Andalusian restaurant"@en .


###  http://www.semanticweb.org/javi/ontologies/2025/3/tir#Beach
:Beach rdf:type owl:Class ;
       rdfs:subClassOf :TouristAttraction ;
       rdfs:comment "Bank of the sea or a large river, formed by sandy beaches on an almost flat surface."@en ;
       rdfs:label "Beach"@en .


###  http://www.semanticweb.org/javi/ontologies/2025/3/tir#BeachHotel
:BeachHotel rdf:type owl:Class ;
            rdfs:subClassOf :Hotel ;
            rdfs:comment "Building planned and equipped to provide accommodation services to people, which is located near a beach."@en ;
            rdfs:label "Beach Hotel"@en .


###  http://www.semanticweb.org/javi/ontologies/2025/3/tir#Bus
:Bus rdf:type owl:Class ;
     rdfs:subClassOf :PublicTransport ;
     rdfs:comment "A vehicle for transporting passengers along fixed routes and with pre-established schedules, designed for general use and accessible to anyone for a fee."@en ;
     rdfs:label "Bus"@en .


###  http://www.semanticweb.org/javi/ontologies/2025/3/tir#BusinessHotel
:BusinessHotel rdf:type owl:Class ;
               rdfs:subClassOf :Hotel ;
               rdfs:comment "A building designed and equipped to provide accommodation services for people, focusing on the needs of business travelers, offering services such as meeting rooms, high-speed internet, and business centers to facilitate productivity."@en ;
               rdfs:label "Business Hotel"@en .


###  http://www.semanticweb.org/javi/ontologies/2025/3/tir#City
:City rdf:type owl:Class ;
      owl:equivalentClass [ rdf:type owl:Restriction ;
                            owl:onProperty :hasGeoCoordinates ;
                            owl:qualifiedCardinality "1"^^xsd:nonNegativeInteger ;
                            owl:onClass :GeoCoordinates
                          ] ;
      rdfs:comment "Class representing a human settlement of considerable size."@en ;
      rdfs:label "City"@en .


###  http://www.semanticweb.org/javi/ontologies/2025/3/tir#CulturalAttraction
:CulturalAttraction rdf:type owl:Class ;
                    rdfs:subClassOf :TouristAttraction ;
                    rdfs:comment "Material and intangible elements that represent the culture of a place, which attract tourists."@en ;
                    rdfs:label "Cultural attraction"@en .


###  http://www.semanticweb.org/javi/ontologies/2025/3/tir#CulturalEvent
:CulturalEvent rdf:type owl:Class ;
               rdfs:subClassOf :Event ;
               rdfs:comment "An organized activity that seeks to promote, celebrate, and disseminate aspects of culture, with the goal of fostering interaction, learning, and connection between people."@en ;
               rdfs:label "Cultural event"@en .


###  http://www.semanticweb.org/javi/ontologies/2025/3/tir#Event
:Event rdf:type owl:Class ;
       rdfs:comment "An important and scheduled social gathering."@en ;
       rdfs:label "Event"@en .


###  http://www.semanticweb.org/javi/ontologies/2025/3/tir#GastronomicEvent
:GastronomicEvent rdf:type owl:Class ;
                  rdfs:subClassOf :Event ;
                  rdfs:comment "Meeting or event where food and drinks are offered to guests."@en ;
                  rdfs:label "Gastronomic event"@en .


###  http://www.semanticweb.org/javi/ontologies/2025/3/tir#GeoCoordinates
:GeoCoordinates rdf:type owl:Class ;
                owl:equivalentClass [ rdf:type owl:Restriction ;
                                      owl:onProperty :isGeoCoordinatesOf ;
                                      owl:qualifiedCardinality "1"^^xsd:nonNegativeInteger ;
                                      owl:onClass :City
                                    ] ;
                rdfs:comment "Reference system that allows each location on Earth to be identified by a pair of numbers that represent latitude and longitude"@en ;
                rdfs:label "Geographic coordinates"@en .


###  http://www.semanticweb.org/javi/ontologies/2025/3/tir#Hotel
:Hotel rdf:type owl:Class ;
       owl:equivalentClass [ rdf:type owl:Restriction ;
                             owl:onProperty :hotelRatingValue ;
                             owl:minQualifiedCardinality "1"^^xsd:nonNegativeInteger ;
                             owl:onDataRange xsd:decimal
                           ] ;
       rdfs:comment "Building planned and equipped to provide accommodation services to people."@en ;
       rdfs:label "Hotel"@en .


###  http://www.semanticweb.org/javi/ontologies/2025/3/tir#ItalianRestaurant
:ItalianRestaurant rdf:type owl:Class ;
                   rdfs:subClassOf :Restaurant ;
                   rdfs:comment "An establishment that offers food and drinks to its customers, generally focusing on Italian cuisine, characterized by dishes such as pasta, pizza, risotto, meats, and desserts, using fresh, quality ingredients."@en ;
                   rdfs:label "Italian restaurant"@en .


###  http://www.semanticweb.org/javi/ontologies/2025/3/tir#JapaneseRestaurant
:JapaneseRestaurant rdf:type owl:Class ;
                    rdfs:subClassOf :Restaurant ;
                    rdfs:comment "Establishment specializing in Japanese cuisine, offering dishes such as sushi, ramen, tempura, yakitori, and others, with an emphasis on fresh ingredients, careful presentation, and natural flavors."@en ;
                    rdfs:label "Japanese restaurant"@en .


###  http://www.semanticweb.org/javi/ontologies/2025/3/tir#LuxuryHotel
:LuxuryHotel rdf:type owl:Class ;
             rdfs:subClassOf :Hotel ;
             rdfs:comment "A building planned and designed to provide accommodation services to people, providing a luxury accommodation experience for the guest."@en ;
             rdfs:label "Luxury Hotel"@en .


###  http://www.semanticweb.org/javi/ontologies/2025/3/tir#MediterraneanRestaurant
:MediterraneanRestaurant rdf:type owl:Class ;
                         rdfs:subClassOf :Restaurant ;
                         rdfs:comment "Public establishment where food and drinks are served, for a fee, to be consumed on the premises, offering dishes based on the Mediterranean diet, characterized by the use of fresh ingredients such as olive oil, vegetables, legumes, fish and seafood, typical of the countries bordering the Mediterranean Sea."@en ;
                         rdfs:label "Mediterranean restaurant"@en .


###  http://www.semanticweb.org/javi/ontologies/2025/3/tir#MexicanRestaurant
:MexicanRestaurant rdf:type owl:Class ;
                   rdfs:subClassOf :Restaurant ;
                   rdfs:comment "A public establishment where food and drinks are served, for a fee, to be consumed on the premises. It offers dishes based on traditional and regional Mexican cuisine, characterized by ingredients such as corn, beans, chili, and a wide variety of sauces and spices."@en ;
                   rdfs:label "Mexican restaurant"@en .


###  http://www.semanticweb.org/javi/ontologies/2025/3/tir#Monument
:Monument rdf:type owl:Class ;
          rdfs:subClassOf :TouristAttraction ;
          rdfs:comment "A building, work of art, or site that has significant historical, artistic, cultural, or scientific value, attracts tourists, and is considered part of a place's cultural heritage."@en ;
          rdfs:label "Monument"@en .


###  http://www.semanticweb.org/javi/ontologies/2025/3/tir#Museum
:Museum rdf:type owl:Class ;
        rdfs:subClassOf :TouristAttraction ;
        rdfs:comment "An institution, generally non-profit and open to the public, that researches, collects, preserves, interprets, and exhibits tangible and intangible heritage, promoting diversity and sustainability."@en ;
        rdfs:label "Museum"@en .


###  http://www.semanticweb.org/javi/ontologies/2025/3/tir#MusicalEvent
:MusicalEvent rdf:type owl:Class ;
              rdfs:subClassOf :Event ;
              rdfs:comment "A gathering or event that brings people together to enjoy live music, which can range from a small concert to a large international festival, with the goal of entertaining, celebrating, or creating shared experiences."@en ;
              rdfs:label "Musical event"@en .


###  http://www.semanticweb.org/javi/ontologies/2025/3/tir#Park
:Park rdf:type owl:Class ;
      rdfs:subClassOf :TouristAttraction ;
      rdfs:comment "A facility designed for the leisure, entertainment, and often recreation of visitors, with attractions, facilities, and activities organized around a central theme or concept."@en ;
      rdfs:label "Park"@en .


###  http://www.semanticweb.org/javi/ontologies/2025/3/tir#PublicBike
:PublicBike rdf:type owl:Class ;
            rdfs:subClassOf :PublicTransport ;
            rdfs:comment "A transportation service that makes bicycles available to the public for temporary use, usually in urban settings, allowing users to pick up a bicycle at one location and return it at another."@en ;
            rdfs:label "Public bike"@en .


###  http://www.semanticweb.org/javi/ontologies/2025/3/tir#PublicTransport
:PublicTransport rdf:type owl:Class ;
                 rdfs:comment "A comprehensive system of transportation, used by the general public, that seeks to satisfy people's mobility needs, unlike private transportation, where the user owns and controls the vehicle."@en ;
                 rdfs:label "Public transport"@en .


###  http://www.semanticweb.org/javi/ontologies/2025/3/tir#Restaurant
:Restaurant rdf:type owl:Class ;
            owl:equivalentClass [ rdf:type owl:Restriction ;
                                  owl:onProperty :restAveragePrice ;
                                  owl:qualifiedCardinality "1"^^xsd:nonNegativeInteger ;
                                  owl:onDataRange xsd:decimal
                                ] ;
            rdfs:comment "A public establishment where food and drinks are served, for a fee, to be consumed on the premises."@en ;
            rdfs:label "Restaurant"@en .


###  http://www.semanticweb.org/javi/ontologies/2025/3/tir#RuralHotel
:RuralHotel rdf:type owl:Class ;
            rdfs:subClassOf :Hotel ;
            rdfs:comment "A building planned and equipped to provide accommodation services to people, located in a rural setting and usually offering complementary services, such as restaurants, activities, or excursions."@en ;
            rdfs:label "Rural Hotel"@en .


###  http://www.semanticweb.org/javi/ontologies/2025/3/tir#SportEvent
:SportEvent rdf:type owl:Class ;
            rdfs:subClassOf :Event ;
            rdfs:comment "An organized activity that involves physical or mental competition among participants. It can range from small local tournaments to international championships, and aims to promote values ​​such as teamwork and personal improvement."@en ;
            rdfs:label "Sport event"@en .


###  http://www.semanticweb.org/javi/ontologies/2025/3/tir#Subway
:Subway rdf:type owl:Class ;
        rdfs:subClassOf :PublicTransport ;
        rdfs:comment "A rail system operating primarily in urban and suburban areas, designed to transport large numbers of passengers quickly and efficiently, via railway tracks segregated from vehicular traffic."@en ;
        rdfs:label "Subway"@en .


###  http://www.semanticweb.org/javi/ontologies/2025/3/tir#Taxi
:Taxi rdf:type owl:Class ;
      rdfs:subClassOf :PublicTransport ;
      rdfs:comment "A vehicle with a driver that provides passenger transportation services, in which the user pays a fee to the driver in exchange for the transportation service provided."@en ;
      rdfs:label "Taxi"@en .


###  http://www.semanticweb.org/javi/ontologies/2025/3/tir#TechnologyEvent
:TechnologyEvent rdf:type owl:Class ;
                 rdfs:subClassOf :Event ;
                 rdfs:comment "Meetings, conferences, trade shows, or congresses, among other formats, where advances, innovations, and developments in technology are presented and discussed, with the aim of promoting knowledge exchange, networking, and innovation."@en ;
                 rdfs:label "Technology event"@en .


###  http://www.semanticweb.org/javi/ontologies/2025/3/tir#TouristAttraction
:TouristAttraction rdf:type owl:Class ;
                   rdfs:comment "Any place, event, or activity that attracts people for its cultural, historical, recreational, or natural value, contributing to the development of tourism."@en ;
                   rdfs:label "Tourist attraction"@en .


###  http://www.semanticweb.org/javi/ontologies/2025/3/tir#TouristHotel
:TouristHotel rdf:type owl:Class ;
              rdfs:subClassOf :Hotel ;
              rdfs:comment "Building planned and equipped to provide accommodation and food services to people"@en ;
              rdfs:label "Tourist Hotel"@en .


###  http://www.semanticweb.org/javi/ontologies/2025/3/tir#Tram
:Tram rdf:type owl:Class ;
      rdfs:subClassOf :PublicTransport ;
      rdfs:comment "A vehicle that runs on rails within or near a city and is used to transport passengers."@en ;
      rdfs:label "Tram"@en .


#################################################################
#    Individuals
#################################################################

###  http://www.semanticweb.org/javi/ontologies/2025/3/tir#city03
:city03 rdf:type owl:NamedIndividual ,
                 :City ,
                 :Event ,
                 :Hotel ,
                 :PublicTransport ;
        :hasGeoCoordinates :coordCity03 ;
        :cityIdentifier "3"^^xsd:int ;
        :cityName "Madrid" ;
        owl:sameAs "http://dbpedia.org/resource/Madrid" .


###  http://www.semanticweb.org/javi/ontologies/2025/3/tir#coordCity03
:coordCity03 rdf:type owl:NamedIndividual ,
                      :GeoCoordinates ;
             :isGeoCoordinatesOf :city03 ;
             :latitude "40.4168"^^xsd:float ;
             :longitude "-3.7038"^^xsd:float .


###  http://www.semanticweb.org/javi/ontologies/2025/3/tir#culturalEvent31
:culturalEvent31 rdf:type owl:NamedIndividual ,
                          :City ,
                          :CulturalEvent ,
                          :Hotel ,
                          :PublicTransport ;
                 :eventLocatedIn :city03 ;
                 :eventIdentifier "31"^^xsd:int ;
                 :eventName "Feria Madrid" ;
                 :startDate "2024-12-18T00:00:00"^^xsd:dateTime .


###  http://www.semanticweb.org/javi/ontologies/2025/3/tir#italianRestaurant85
:italianRestaurant85 rdf:type owl:NamedIndividual ,
                              :City ,
                              :Event ,
                              :Hotel ,
                              :ItalianRestaurant ,
                              :PublicTransport ;
                     :restLocatedIn :city03 ;
                     :restAveragePrice 43.0 ;
                     :restIdentifier "85"^^xsd:int ;
                     :restName "Restaurante Fusión Madrid" ;
                     :restRatingValue 4.6 ;
                     owl:sameAs "http://dbpedia.org/resource/Italian_cuisine" .


###  http://www.semanticweb.org/javi/ontologies/2025/3/tir#luxuryHotel68
:luxuryHotel68 rdf:type owl:NamedIndividual ,
                        :City ,
                        :Event ,
                        :LuxuryHotel ,
                        :PublicTransport ;
               :hotelLocatedIn :city03 ;
               :hotelIdentifier "68"^^xsd:int ;
               :hotelName "Hotel Del Mar Madrid" ;
               :hotelRatingValue 3.8 ;
               :pricePerNight 172.0 ;
               :starRating "3"^^xsd:int .


###  http://www.semanticweb.org/javi/ontologies/2025/3/tir#monument74
:monument74 rdf:type owl:NamedIndividual ,
                     :City ,
                     :Event ,
                     :Hotel ,
                     :Monument ,
                     :PublicTransport ;
            :tourLocatedIn :city03 ;
            :tourIdentifier "74"^^xsd:int ;
            :tourName "Palacio Madrid" ;
            :tourRatingValue 4.6 ;
            owl:sameAs "http://dbpedia.org/resource/Royal_Palace_of_Madrid" .


###  http://www.semanticweb.org/javi/ontologies/2025/3/tir#publicBike82
:publicBike82 rdf:type owl:NamedIndividual ,
                       :City ,
                       :Event ,
                       :Hotel ,
                       :PublicTransport ;
              :transLocatedIn :city03 ;
              :legalName "City Madrid" ;
              :transAveragePrice 68.0 ;
              :transIdentifier "82"^^xsd:int .


#################################################################
#    Rules
#################################################################

<http://www.semanticweb.org/javi/ontologies/2025/3/tir/h> rdf:type <http://www.w3.org/2003/11/swrl#Variable> .

<http://www.semanticweb.org/javi/ontologies/2025/3/tir/e> rdf:type <http://www.w3.org/2003/11/swrl#Variable> .

<http://www.semanticweb.org/javi/ontologies/2025/3/tir/v> rdf:type <http://www.w3.org/2003/11/swrl#Variable> .

<http://www.semanticweb.org/javi/ontologies/2025/3/tir/m> rdf:type <http://www.w3.org/2003/11/swrl#Variable> .

<http://www.semanticweb.org/javi/ontologies/2025/3/tir/r> rdf:type <http://www.w3.org/2003/11/swrl#Variable> .

<http://www.semanticweb.org/javi/ontologies/2025/3/tir/n> rdf:type <http://www.w3.org/2003/11/swrl#Variable> .

[ <http://swrl.stanford.edu/ontologies/3.3/swrla.owl#isRuleEnabled> "true"^^xsd:boolean ;
   rdfs:comment "All museums have a rating greater than 3.5" ;
   rdfs:label "RuleMuseumRating" ;
   rdf:type <http://www.w3.org/2003/11/swrl#Imp> ;
   <http://www.w3.org/2003/11/swrl#body> [ rdf:type <http://www.w3.org/2003/11/swrl#AtomList> ;
                                           rdf:first [ rdf:type <http://www.w3.org/2003/11/swrl#ClassAtom> ;
                                                       <http://www.w3.org/2003/11/swrl#classPredicate> :Museum ;
                                                       <http://www.w3.org/2003/11/swrl#argument1> <http://www.semanticweb.org/javi/ontologies/2025/3/tir/m>
                                                     ] ;
                                           rdf:rest [ rdf:type <http://www.w3.org/2003/11/swrl#AtomList> ;
                                                      rdf:first [ rdf:type <http://www.w3.org/2003/11/swrl#DatavaluedPropertyAtom> ;
                                                                  <http://www.w3.org/2003/11/swrl#propertyPredicate> :tourRatingValue ;
                                                                  <http://www.w3.org/2003/11/swrl#argument1> <http://www.semanticweb.org/javi/ontologies/2025/3/tir/m> ;
                                                                  <http://www.w3.org/2003/11/swrl#argument2> <http://www.semanticweb.org/javi/ontologies/2025/3/tir/v>
                                                                ] ;
                                                      rdf:rest [ rdf:type <http://www.w3.org/2003/11/swrl#AtomList> ;
                                                                 rdf:first [ rdf:type <http://www.w3.org/2003/11/swrl#BuiltinAtom> ;
                                                                             <http://www.w3.org/2003/11/swrl#builtin> <http://www.w3.org/2003/11/swrlb#greaterThan> ;
                                                                             <http://www.w3.org/2003/11/swrl#arguments> [ rdf:type rdf:List ;
                                                                                                                          rdf:first <http://www.semanticweb.org/javi/ontologies/2025/3/tir/v> ;
                                                                                                                          rdf:rest [ rdf:type rdf:List ;
                                                                                                                                     rdf:first 3.5 ;
                                                                                                                                     rdf:rest rdf:nil
                                                                                                                                   ]
                                                                                                                        ]
                                                                           ] ;
                                                                 rdf:rest rdf:nil
                                                               ]
                                                    ]
                                         ] ;
   <http://www.w3.org/2003/11/swrl#head> [ rdf:type <http://www.w3.org/2003/11/swrl#AtomList> ;
                                           rdf:first [ rdf:type <http://www.w3.org/2003/11/swrl#ClassAtom> ;
                                                       <http://www.w3.org/2003/11/swrl#classPredicate> :Museum ;
                                                       <http://www.w3.org/2003/11/swrl#argument1> <http://www.semanticweb.org/javi/ontologies/2025/3/tir/m>
                                                     ] ;
                                           rdf:rest rdf:nil
                                         ]
 ] .

[ <http://swrl.stanford.edu/ontologies/3.3/swrla.owl#isRuleEnabled> "true"^^xsd:boolean ;
   rdfs:comment "All restaurants with gourmet in their names have a 3.5 or greater rating value" ;
   rdfs:label "RuleRestaurantRating" ;
   rdf:type <http://www.w3.org/2003/11/swrl#Imp> ;
   <http://www.w3.org/2003/11/swrl#body> [ rdf:type <http://www.w3.org/2003/11/swrl#AtomList> ;
                                           rdf:first [ rdf:type <http://www.w3.org/2003/11/swrl#ClassAtom> ;
                                                       <http://www.w3.org/2003/11/swrl#classPredicate> :Restaurant ;
                                                       <http://www.w3.org/2003/11/swrl#argument1> <http://www.semanticweb.org/javi/ontologies/2025/3/tir/r>
                                                     ] ;
                                           rdf:rest [ rdf:type <http://www.w3.org/2003/11/swrl#AtomList> ;
                                                      rdf:first [ rdf:type <http://www.w3.org/2003/11/swrl#DatavaluedPropertyAtom> ;
                                                                  <http://www.w3.org/2003/11/swrl#propertyPredicate> :restName ;
                                                                  <http://www.w3.org/2003/11/swrl#argument1> <http://www.semanticweb.org/javi/ontologies/2025/3/tir/r> ;
                                                                  <http://www.w3.org/2003/11/swrl#argument2> <http://www.semanticweb.org/javi/ontologies/2025/3/tir/n>
                                                                ] ;
                                                      rdf:rest [ rdf:type <http://www.w3.org/2003/11/swrl#AtomList> ;
                                                                 rdf:first [ rdf:type <http://www.w3.org/2003/11/swrl#BuiltinAtom> ;
                                                                             <http://www.w3.org/2003/11/swrl#builtin> <http://www.w3.org/2003/11/swrlb#containsIgnoreCase> ;
                                                                             <http://www.w3.org/2003/11/swrl#arguments> [ rdf:type rdf:List ;
                                                                                                                          rdf:first <http://www.semanticweb.org/javi/ontologies/2025/3/tir/n> ;
                                                                                                                          rdf:rest [ rdf:type rdf:List ;
                                                                                                                                     rdf:first "Gourmet" ;
                                                                                                                                     rdf:rest rdf:nil
                                                                                                                                   ]
                                                                                                                        ]
                                                                           ] ;
                                                                 rdf:rest [ rdf:type <http://www.w3.org/2003/11/swrl#AtomList> ;
                                                                            rdf:first [ rdf:type <http://www.w3.org/2003/11/swrl#DatavaluedPropertyAtom> ;
                                                                                        <http://www.w3.org/2003/11/swrl#propertyPredicate> :restRatingValue ;
                                                                                        <http://www.w3.org/2003/11/swrl#argument1> <http://www.semanticweb.org/javi/ontologies/2025/3/tir/r> ;
                                                                                        <http://www.w3.org/2003/11/swrl#argument2> <http://www.semanticweb.org/javi/ontologies/2025/3/tir/v>
                                                                                      ] ;
                                                                            rdf:rest [ rdf:type <http://www.w3.org/2003/11/swrl#AtomList> ;
                                                                                       rdf:first [ rdf:type <http://www.w3.org/2003/11/swrl#BuiltinAtom> ;
                                                                                                   <http://www.w3.org/2003/11/swrl#builtin> <http://www.w3.org/2003/11/swrlb#greaterThanOrEqual> ;
                                                                                                   <http://www.w3.org/2003/11/swrl#arguments> [ rdf:type rdf:List ;
                                                                                                                                                rdf:first <http://www.semanticweb.org/javi/ontologies/2025/3/tir/v> ;
                                                                                                                                                rdf:rest [ rdf:type rdf:List ;
                                                                                                                                                           rdf:first 3.5 ;
                                                                                                                                                           rdf:rest rdf:nil
                                                                                                                                                         ]
                                                                                                                                              ]
                                                                                                 ] ;
                                                                                       rdf:rest rdf:nil
                                                                                     ]
                                                                          ]
                                                               ]
                                                    ]
                                         ] ;
   <http://www.w3.org/2003/11/swrl#head> [ rdf:type <http://www.w3.org/2003/11/swrl#AtomList> ;
                                           rdf:first [ rdf:type <http://www.w3.org/2003/11/swrl#ClassAtom> ;
                                                       <http://www.w3.org/2003/11/swrl#classPredicate> :Restaurant ;
                                                       <http://www.w3.org/2003/11/swrl#argument1> <http://www.semanticweb.org/javi/ontologies/2025/3/tir/r>
                                                     ] ;
                                           rdf:rest rdf:nil
                                         ]
 ] .

[ <http://swrl.stanford.edu/ontologies/3.3/swrla.owl#isRuleEnabled> "true"^^xsd:boolean ;
   rdfs:comment "Hotels with 4 or more stars have a valoration greater than 3.5" ;
   rdfs:label "RuleValorationHotel" ;
   rdf:type <http://www.w3.org/2003/11/swrl#Imp> ;
   <http://www.w3.org/2003/11/swrl#body> [ rdf:type <http://www.w3.org/2003/11/swrl#AtomList> ;
                                           rdf:first [ rdf:type <http://www.w3.org/2003/11/swrl#ClassAtom> ;
                                                       <http://www.w3.org/2003/11/swrl#classPredicate> :Hotel ;
                                                       <http://www.w3.org/2003/11/swrl#argument1> <http://www.semanticweb.org/javi/ontologies/2025/3/tir/h>
                                                     ] ;
                                           rdf:rest [ rdf:type <http://www.w3.org/2003/11/swrl#AtomList> ;
                                                      rdf:first [ rdf:type <http://www.w3.org/2003/11/swrl#DatavaluedPropertyAtom> ;
                                                                  <http://www.w3.org/2003/11/swrl#propertyPredicate> :starRating ;
                                                                  <http://www.w3.org/2003/11/swrl#argument1> <http://www.semanticweb.org/javi/ontologies/2025/3/tir/h> ;
                                                                  <http://www.w3.org/2003/11/swrl#argument2> <http://www.semanticweb.org/javi/ontologies/2025/3/tir/e>
                                                                ] ;
                                                      rdf:rest [ rdf:type <http://www.w3.org/2003/11/swrl#AtomList> ;
                                                                 rdf:first [ rdf:type <http://www.w3.org/2003/11/swrl#BuiltinAtom> ;
                                                                             <http://www.w3.org/2003/11/swrl#builtin> <http://www.w3.org/2003/11/swrlb#greaterThanOrEqual> ;
                                                                             <http://www.w3.org/2003/11/swrl#arguments> [ rdf:type rdf:List ;
                                                                                                                          rdf:first <http://www.semanticweb.org/javi/ontologies/2025/3/tir/e> ;
                                                                                                                          rdf:rest [ rdf:type rdf:List ;
                                                                                                                                     rdf:first 4 ;
                                                                                                                                     rdf:rest rdf:nil
                                                                                                                                   ]
                                                                                                                        ]
                                                                           ] ;
                                                                 rdf:rest [ rdf:type <http://www.w3.org/2003/11/swrl#AtomList> ;
                                                                            rdf:first [ rdf:type <http://www.w3.org/2003/11/swrl#DatavaluedPropertyAtom> ;
                                                                                        <http://www.w3.org/2003/11/swrl#propertyPredicate> :hotelRatingValue ;
                                                                                        <http://www.w3.org/2003/11/swrl#argument1> <http://www.semanticweb.org/javi/ontologies/2025/3/tir/h> ;
                                                                                        <http://www.w3.org/2003/11/swrl#argument2> <http://www.semanticweb.org/javi/ontologies/2025/3/tir/v>
                                                                                      ] ;
                                                                            rdf:rest [ rdf:type <http://www.w3.org/2003/11/swrl#AtomList> ;
                                                                                       rdf:first [ rdf:type <http://www.w3.org/2003/11/swrl#BuiltinAtom> ;
                                                                                                   <http://www.w3.org/2003/11/swrl#builtin> <http://www.w3.org/2003/11/swrlb#greaterThan> ;
                                                                                                   <http://www.w3.org/2003/11/swrl#arguments> [ rdf:type rdf:List ;
                                                                                                                                                rdf:first <http://www.semanticweb.org/javi/ontologies/2025/3/tir/v> ;
                                                                                                                                                rdf:rest [ rdf:type rdf:List ;
                                                                                                                                                           rdf:first 3.5 ;
                                                                                                                                                           rdf:rest rdf:nil
                                                                                                                                                         ]
                                                                                                                                              ]
                                                                                                 ] ;
                                                                                       rdf:rest rdf:nil
                                                                                     ]
                                                                          ]
                                                               ]
                                                    ]
                                         ] ;
   <http://www.w3.org/2003/11/swrl#head> [ rdf:type <http://www.w3.org/2003/11/swrl#AtomList> ;
                                           rdf:first [ rdf:type <http://www.w3.org/2003/11/swrl#ClassAtom> ;
                                                       <http://www.w3.org/2003/11/swrl#classPredicate> :Hotel ;
                                                       <http://www.w3.org/2003/11/swrl#argument1> <http://www.semanticweb.org/javi/ontologies/2025/3/tir/h>
                                                     ] ;
                                           rdf:rest rdf:nil
                                         ]
 ] .

###  Generated by the OWL API (version 5.1.18) https://github.com/owlcs/owlapi/
